DinD: basic support for `if` statements
This exists mostly to ensure that statement translation is fully
fleshed-out.

Source/DafnyCompilers/minimal.cs
@@ -1,3 +1,8 @@
 DafnyRuntime.Helpers.Print(new BigInteger(1));
 DafnyRuntime.Helpers.Print("A");
 DafnyRuntime.Helpers.Print(DafnyRuntime.Sequence<>.FromElements(new BigInteger(1), (new BigInteger(2) + new BigInteger(3)), new BigInteger(4)));
+if ((true && false)) {
+  DafnyRuntime.Helpers.Print("true");
+} else {
+  DafnyRuntime.Helpers.Print("false");
+}
