Source/DafnyCompilers/minimal.dfy
@@ -2,4 +2,9 @@ method Main() {
   print(1);
   print("A");
   print([1,2+3,4]);
+  if true && false {
+    print("true");
+  } else {
+    print("false");
+  }
 }
